theories/NormalEq.v
@@ -40,6 +40,7 @@ match t with
 | tId A t u => noccurn n A && noccurn n t && noccurn n u
 | tRefl A t => noccurn n A && noccurn n t
 | tIdElim A x P hr y t => noccurn n A && noccurn n x && noccurn (S (S n)) P && noccurn n hr && noccurn n y && noccurn n t
+| tQuote t => noccurn n t
 end.
 
 Lemma noccurn_ren_id : forall n t ρ, (forall m, m <> n -> ρ m = m) -> noccurn n t -> t⟨ρ⟩ = t.
@@ -131,6 +132,7 @@ Fixpoint erase (t : term) := match t with
 | tId A t u => tId (erase A) (erase t) (erase u)
 | tRefl A t => tRefl (erase A) (erase t)
 | tIdElim A x P hr y t => tIdElim (erase A) (erase x) (erase P) (erase hr) (erase y) (erase t)
+| tQuote t => tQuote (erase t)
 end.
 
 Definition eqnf t u := erase t = erase u.
